# Section I.5
## Exercise 14
If $N_1 \triangleleft G_1, N_2 \triangleleft G_2$ then $(N_1 \times N_2) \triangleleft(G_1 \times G_2)$ and $(G_1 \times G_2) /(N_1 \times N_2) \cong(G_1 / N_1) \times(G_2 / N_2)$.

Proof

For all $(g_1,g_2)\in G_1\times G_2$, for all $(n_1,n_2)\in N_1\times N_2$ we have $(g_1,g_2)(n_1,n_2)(g_1,g_2)^{-1}=(g_1n_1g_1^{-1},g_2n_2g_2^{-1})\in N_1\times N_2$

So $(N_1 \times N_2) \triangleleft(G_1 \times G_2)$.

Consider the homomorphism $G_1 \times G_2 \to G_1/N_1,(g_1,g_2)\mapsto g_1N_1$ and the homomorphism $G_1 \times G_2 \to G_1/N_1,(g_1,g_2)\mapsto g_2N_2$.

By Universal Mapping Property we get a homomorphism $\phi: G_1 \times G_2 \to (G_1/N_1) \times (G_2/N_2)$.

Then $(g_1,g_2)\in\ker\phi\iff g_1N_1=N_1\land g_2N_2=N_2\iff g_1\in N_1\land g_2\in N_2$.

By First Isomorphism Theorem, so $\ker\phi=N_1\times N_2$.

# Section I.6
## Exercise 11
Find all normal subgroups of $D_n$.

Solution

Let $N$ be a normal subgroup of $D_n$. Then $N \cap C_n$ is a normal subgroup of $C_n$, where $C_n=\langle r \rangle$ is the cyclic subgroup of $D_n$ generated by $r$. The normal subgroups of $C_n$ are precisely the subgroups $\langle r^d \rangle$ for each divisor $d$ of $n$. Thus, $N \cap C_n = \langle r^d \rangle$ for some divisor $d$ of $n$.

For all $j$, we have $a(a^j b) a^{-1}=a^{j+2} b$, so if $N$ contains any reflection $a^j b$, then it contains $a^{j+2k} b$ for all $k$. If $n$ is even, then $N$ may contain either all reflections of the form $a^{2k} b$ or all reflections of the form $a^{2k+1} b$, or all reflections. If $n$ is odd, then $N$ must contain all reflections. So the normal subgroups of $D_n$ are:

For all divisors $d$ of $n$:
1.  If $n$ is odd, the subgroups $\langle r^d \rangle$ and $\langle r^d, s \rangle$.
2.  If $n$ is even, the subgroups $\langle r^d \rangle$ and $\langle r^d, s \rangle$ and $\langle r^d, rs \rangle$.

# Section I.8
## Exercise 2
Give an example of groups $H_i, K_j$ such that $H_1 \times H_2 \cong K_1 \times K_2$ and no $H_i$ is isomorphic to any $K_j$.

Proof

Let $H_1 = \mathbb{Z}_2 \times \mathbb{Z}_3$, $`H_2 = \{e\}`$, $K_1 = \mathbb{Z}_2$, and $K_2 = \mathbb{Z}_3$.

First, we show $H_1 \times H_2 \cong K_1 \times K_2$:
$H_1 \times H_2 = (\mathbb{Z}_2 \times \mathbb{Z}_3) \times \{e\} \cong \mathbb{Z}_2 \times \mathbb{Z}_3$.
Since $K_1 \times K_2 = \mathbb{Z}_2 \times \mathbb{Z}_3$, the products are isomorphic.
By the Chinese Remainder Theorem, both products are isomorphic to $\mathbb{Z}_6$.

Next, we show no $H_i$ is isomorphic to any $K_j$. We can do this by comparing their orders:
- $|H_1| = |\mathbb{Z}_2 \times \mathbb{Z}_3| = 6$
- $`|H_2| = |\{e\}| = 1`$
- $|K_1| = |\mathbb{Z}_2| = 2$
- $|K_2| = |\mathbb{Z}_3| = 3$

Since all four groups have different orders, no two of them can be isomorphic. Therefore, no $H_i$ is isomorphic to any $K_j$.

## Exercise 3
Let $G$ be an (additive) abelian group with subgroups $H$ and $K$. Show that $G \cong H \oplus K$ if and only if there are homomorphisms $H \overunderset{\pi_1}{\iota_1}{\leftrightarrows} G \overunderset{\pi_2}{\iota_2}{\rightleftarrows} K$ such that $\pi_1 \iota_1=1_H, \pi_2 \iota_2=1_K, \pi_1 \iota_2=0$ and $\pi_2 \iota_1=0$, where 0 is the map sending every element onto the zero (identity) element, and $\iota_1 \pi_1(x)+\iota_2 \pi_2(x)=x$ for all $x \in G$.

Proof

($\Rightarrow$) Suppose $G \cong H \oplus K$. Then every element $g \in G$ can be uniquely expressed as $g = h + k$ for some $h \in H$ and $k \in K$. Define the homomorphisms $\iota_1: H \to G$ by $\iota_1(h) = h$, $\iota_2: K \to G$ by $\iota_2(k) = k$, $\pi_1: G \to H$ by $\pi_1(h + k) = h$, and $\pi_2: G \to K$ by $\pi_2(h + k) = k$. It is straightforward to verify that these maps satisfy the required properties.

($\Leftarrow$) Conversely, suppose we have homomorphisms $\iota_1, \iota_2, \pi_1, \pi_2$ satisfying the given conditions. Define a map $\phi: H \oplus K \to G$ by $\phi(h, k) = \iota_1(h) + \iota_2(k)$. This map is a homomorphism: $\phi(h_1, k_1) + \phi(h_2, k_2) = \iota_1(h_1) + \iota_2(k_1) + \iota_1(h_2) + \iota_2(k_2) = \iota_1(h_1 + h_2) + \iota_2(k_1 + k_2) = \phi(h_1 + h_2, k_1 + k_2)$.

Define $\psi: G \to H \oplus K$ by $\psi(g) = (\pi_1(g), \pi_2(g))$. Then $\psi(\phi(h, k)) = \psi(\iota_1(h) + \iota_2(k)) = (\pi_1(\iota_1(h) + \iota_2(k)), \pi_2(\iota_1(h) + \iota_2(k))) = (h, k)$, and $\phi(\psi(g)) = \phi(\pi_1(g), \pi_2(g)) = \iota_1(\pi_1(g)) + \iota_2(\pi_2(g)) = g$. Thus, $\phi$ is an isomorphism, and $G \cong H \oplus K$.

## Exercise 5
Let $G, H$ be finite cyclic groups. Then $G \times H$ is cyclic if and only if $(|G|,|H|)=1$.

Proof

Suppose $G=\langle g \rangle$ and $H=\langle h \rangle$.

If $(|G|,|H|)=1$, then the order of $(g,h)$ is $\mathrm{lcm}(|G|,|H|)=|G||H|$, so $(g,h)$ generates $G \times H$.

Conversely, if $G \times H$ is cyclic, it is generated by an element $(g^a, h^b)$. The projections of this generator must generate $G$ and $H$ respectively, so $\langle g^a \rangle = G$ and $\langle h^b \rangle = H$. This implies $\gcd(a, |G|) = 1$ and $\gcd(b, |H|) = 1$. The order of $(g^a, h^b)$ is then $\mathrm{lcm}(\mathrm{ord}(g^a), \mathrm{ord}(h^b)) = \mathrm{lcm}(|G|, |H|)$. For this to be $|G||H|$, it must be that $\gcd(|G|, |H|) = 1$.

## Exercise 9
If a group $G$ is the (internal) direct product of its subgroups $H, K$, then $H \cong G / K$ and $G / H \cong K$.

Proof

Define a map $\pi_H: G \to H$ for $g=hk$ (with unique $h \in H, k \in K$) by $\pi_H(g) = h$. This is a surjective homomorphism with kernel $K$. By the First Isomorphism Theorem, $G/K \cong H$.

Similarly, the projection $\pi_K: G \to K$ given by $\pi_K(hk)=k$ is a surjective homomorphism with kernel $H$, so $G/H \cong K$.

# Section I.9
## Exercise 1
Every nonidentity element in a free group $F$ has infinite order.

Proof

Let $w$ be a reduced nonidentity word in $F$ of minimal length with finite order, and let $n>1$ be such that $w^n=1$. In the product $w^n = w \cdots w$, since $w$ is reduced, any cancellation must occur between adjacent copies of $w$. This means the last letter of $w$ must be the inverse of the first letter of $w$. So we can write $w=a u a^{-1}$ for some letter $a$ and some word $u$. Then $w^n=(a u a^{-1})^n = a u^n a^{-1}$, so $u^n=1$. Since $u$ is shorter than $w$, by minimality we must have $u=1$. This implies $w=aa^{-1}=1$, which contradicts $w$ being a nonidentity element.

## Exercise 4
Let $F$ be the free group on the set $X$, and let $Y \subset X$. If $H$ is the smallest normal subgroup of $F$ containing $Y$, then $F / H$ is a free group.

Proof

Let $Z=X \setminus Y$. Define a map $\phi: X \to F(Z)$ by $\phi(x)=x$ if $x \in Z$ and $\phi(x)=1$ if $x \in Y$. By the Universal Mapping Property of free groups, $\phi$ extends to a homomorphism $\tilde{\phi}: F(X) \to F(Z)$. Since $\tilde{\phi}(y)=1$ for all $y \in Y$, the smallest normal subgroup containing $Y$, $H$, is contained in $\ker(\tilde{\phi})$. Thus, $\tilde{\phi}$ induces a homomorphism $\bar{\phi}: F(X)/H \to F(Z)$.

To show this is an isomorphism, we construct an inverse. Let $\psi: Z \to F(X)/H$ be the map $\psi(z) = zH$. By the Universal Mapping Property of $F(Z)$, this extends to a homomorphism $\tilde{\psi}: F(Z) \to F(X)/H$. We check that $\bar{\phi}$ and $\tilde{\psi}$ are inverses. For any $z \in Z$, $\bar{\phi}(\tilde{\psi}(z)) = \bar{\phi}(zH) = \tilde{\phi}(z) = z$. For any $x \in X$, if $x \in Z$, $\tilde{\psi}(\bar{\phi}(xH)) = \tilde{\psi}(x) = xH$. If $x \in Y$, $\tilde{\psi}(\bar{\phi}(xH)) = \tilde{\psi}(1) = H$, and since $x \in Y \subseteq H$, $xH=H$. Since the compositions are the identity on the generating sets, they are identity homomorphisms. Thus $F(X)/H \cong F(Z)$, and so $F(X)/H$ is a free group on the set $Z$.
